\documentclass[11pt,reqno]{amsart}
\usepackage{geometry}                % See geometry.pdf to learn the layout options. There are lots.
\geometry{letterpaper}                   % ... or a4paper or a5paper or ... 
%\geometry{landscape}                % Activate for for rotated page geometry
%\usepackage[parfill]{parskip}    % Activate to begin paragraphs with an empty line rather than an indent
\usepackage{graphicx}
\usepackage{amssymb}
\usepackage[all]{xy}
\usepackage{epstopdf}
\usepackage{color}
\DeclareGraphicsRule{.tif}{png}{.png}{`convert #1 `dirname #1`/`basename #1 .tif`.png}


% these packages make it easy to include figures in the text. 
\usepackage{float}
\restylefloat{figure}
% newcommand

\begin{document}
%Transformation:
%\begin{equation}
%\begin{split}
%x_1 &= a + b\\
%x_2 &= r\cos\theta\\
%y_1 &= r\sin\theta\\
%y_2 &= -a + b^3
%\end{split}
%\end{equation}
%Derivative of transformation:
%\begin{equation}
%\begin{split}
%\dot{x}_1 &= \dot{a} +\dot{b}\\
%\dot{x}_2 &= \dot{r}\cos\theta -  r\dot{\theta}\sin\theta\\
%\dot{y}_1 &= \dot{r}\sin\theta +  r\dot{\theta}\cos\theta\\
%\dot{y}_2 &= -\dot{a} + 3b^2\dot{b}
%\end{split}
%\end{equation}
Dynamics:
\begin{equation}
\begin{split}
\dot{x}_1 &= x_2\\
\dot{x}_2 &= -y_1^2x_1^3\\
\dot{y}_1 &= y_2\\
\dot{y}_2 &= -\epsilon^{-1}y_1 - \delta y_1^3
\end{split}
\end{equation}
%Transformed dynamics:
%\begin{equation}
%\begin{split}
%\dot{a} +\dot{b} &=  r\cos\theta\\
%\dot{r}\cos\theta -  r\dot{\theta}\sin\theta &= -\left( r\sin\theta\right)^2( a + b)^3\\
%\dot{r}\sin\theta +  r\dot{\theta}\cos\theta&=  -a + b^3\\
%-\dot{a} + 3b^2\dot{b} &= -\epsilon^{-1}\left( r\sin\theta\right) - \delta \left( r\sin\theta\right)^3
%\end{split}
%\end{equation}
%Solve for $\dot{a},\dot{b},\dot{r},\dot{\theta}$:
%%\begin{equation}
%%\begin{split}
%%\dot{b} + 3b^2\dot{b} &=  r\cos\theta -\epsilon^{-1}\left( r\sin\theta\right) - \delta \left( r\sin\theta\right)^3\\
%%\dot{b}&= \frac{ r\cos\theta -\epsilon^{-1}r\sin\theta - \delta \left( r\sin\theta\right)^3}{1+3b^2}\\
%%\end{split}
%%\end{equation}
%%
%%\begin{equation}
%%\begin{split}
%%\dot{a} &= r\cos\theta - \frac{ r\cos\theta -\epsilon^{-1}r\sin\theta - \delta \left( r\sin\theta\right)^3}{1+3b^2}\\
%%&= \frac{ 3b^2 r\cos\theta  +\epsilon^{-1}r\sin\theta + \delta \left( r\sin\theta\right)^3}{1+3b^2}\\
%%\end{split}
%%\end{equation}
%%
%%\begin{equation}
%%\begin{split}
%%\dot{r} -  r\dot{\theta}\tan\theta &= -\frac{\left( r\sin\theta\right)^2( a + b)^3}{\cos\theta}\\
%%\dot{r} +  r\dot{\theta}\cot\theta&=  \frac{-a + b^3}{\sin\theta}\\
%%\end{split}
%%\end{equation}
%%\begin{equation}
%%\begin{split}
%% r\dot{\theta}\left(\cot\theta +\tan\theta\right)  &=  \frac{-a + b^3}{\sin\theta} + \frac{\left( r\sin\theta\right)^2( a + b)^3}{\cos\theta}\\
%% r\dot{\theta}\left(\frac{\cos^2\theta}{\sin\theta\cos\theta} +\frac{\sin^2\theta}{\sin\theta\cos\theta}\right)  &=  \frac{-a + b^3}{\sin\theta} + \frac{\left( r\sin\theta\right)^2( a + b)^3}{\cos\theta}\\
%%\dot{\theta}\left(\frac{r}{\sin\theta\cos\theta}\right)  &=  \frac{-a + b^3}{\sin\theta} + \frac{\left( r\sin\theta\right)^2( a + b)^3}{\cos\theta}\\
%%\dot{\theta} &= \left(\frac{\sin\theta\cos\theta}{r}\right)  \left( \frac{-a + b^3}{\sin\theta} + \frac{\left( r\sin\theta\right)^2( a + b)^3}{\cos\theta}\right)\\
%%&= \left(\frac{1}{r}\right)  \left[\left( -a + b^3\right)\cos\theta + \left( r\sin\theta\right)^2( a + b)^3\sin\theta\right]\\
%%&= \frac{\left( -a + b^3\right)\cos\theta + r^2\sin^3\theta( a + b)^3}{r}\\
%%\end{split}
%%\end{equation}
%%
%%\begin{equation}
%%\begin{split}
%%\dot{r} &=  \frac{-a + b^3}{\sin\theta} -  \left[\left( -a + b^3\right)\cos\theta + r^2\sin^3\theta( a + b)^3\right]\cot\theta\\
%%&=  \frac{-a + b^3}{\sin\theta} -  \left[\left( -a + b^3\right)\frac{\cos^2\theta}{\sin\theta} + r^2\sin^2\theta\cos\theta( a + b)^3\right]\\
%%&=  \frac{\left( -a + b^3\right)}{\sin\theta}\left(1-\cos^2\theta\right) - r^2\sin^2\theta\cos\theta( a + b)^3\\
%%&= \left( -a + b^3\right)\sin\theta - r^2\sin^2\theta\cos\theta( a + b)^3\\
%%&=\sin\theta\left( \left( -a + b^3\right) - r^2\sin\theta\cos\theta( a + b)^3\right)\\
%%\end{split}
%%\end{equation}
%
%\begin{equation}
%\begin{split}
%\dot{a} &= \frac{ 3b^2 r\cos\theta  +\epsilon^{-1}r\sin\theta + \delta \left( r\sin\theta\right)^3}{1+3b^2}\\
%\dot{b}&= \frac{ r\cos\theta -\epsilon^{-1}r\sin\theta - \delta \left( r\sin\theta\right)^3}{1+3b^2}\\
%\dot{r} &=\sin\theta\left( \left( -a + b^3\right) - r^2\sin\theta\cos\theta( a + b)^3\right)\\
%\dot{\theta} &= \frac{\left( -a + b^3\right)\cos\theta + r^2\sin^3\theta( a + b)^3}{r}\\
%\end{split}
%\end{equation}
%
%Polynomial approximation (approx. up to 3rd order):
%
%\begin{equation}
%\begin{split}
%\dot{a} &= \frac{ 3b^2 r  +\epsilon^{-1}r\theta + \delta \left( r\theta\right)^3}{1+3b^2}\\
%\dot{b}&= \frac{ r\cos\theta -\epsilon^{-1}r\sin\theta - \delta \left( r\sin\theta\right)^3}{1+3b^2}\\
%\dot{r} &=\sin\theta\left( \left( -a + b^3\right) - r^2\sin\theta\cos\theta( a + b)^3\right)\\
%\dot{\theta} &= \frac{\left( -a + b^3\right)\cos\theta + r^2\sin^3\theta( a + b)^3}{r}\\
%\end{split}
%\end{equation}
%
%%\begin{equation}
%%\begin{split}
%%\left[\begin{matrix} \dot{a} \\ \dot{b} \\ \dot{r} \\ \dot{\theta}\end{matrix}\right] \approx
%%\left[\begin{matrix} \end{matrix}\right]
%%\left[\begin{matrix} a\\ b\\ r\\ \theta\end{matrix}\right]
%%\end{split}
%%\end{equation}


\end{document}  
